pulse/lib/pulse/lib/Pulse.Lib.HigherArray.Core.fst
@@ -480,21 +480,21 @@ ghost fn gsub_elim u#a (#t: Type u#a) (arr: array t) #f (#mask: nat->prop) (i j:
 }
 
 unobservable
-fn sub u#a (#t: Type u#a) (arr: array t) #f #mask (i: SZ.t) (j: SZ.t)
-    (#v: erased (Seq.seq t) { SZ.v i <= SZ.v j /\ SZ.v j <= Seq.length (reveal v) })
+fn sub u#a (#t: Type u#a) (arr: array t) #f #mask (i: SZ.t) (j: erased nat)
+    (#v: erased (Seq.seq t) { SZ.v i <= j /\ j <= Seq.length (reveal v) })
   requires pts_to_mask arr #f v mask
   returns sub: (sub: array t { length arr == Seq.length (reveal v) })
-  ensures rewrites_to sub (gsub arr (SZ.v i) (SZ.v j))
-  ensures pts_to_mask sub #f (Seq.slice v (SZ.v i) (SZ.v j)) (fun k -> mask (k + SZ.v i))
-  ensures pts_to_mask arr #f v (fun k -> mask k /\ ~(SZ.v i <= k /\ k < SZ.v j))
+  ensures rewrites_to sub (gsub arr (SZ.v i) j)
+  ensures pts_to_mask sub #f (Seq.slice v (SZ.v i) j) (fun k -> mask (k + SZ.v i))
+  ensures pts_to_mask arr #f v (fun k -> mask k /\ ~(SZ.v i <= k /\ k < j))
 {
-  let pred = (fun k -> SZ.v i <= k /\ k < SZ.v j);
+  let pred = (fun k -> SZ.v i <= k /\ k < j);
   pts_to_mask_props arr;
   split_mask arr pred;
-  gsub_intro arr #f #(mask_isect mask pred) (SZ.v i) (SZ.v j);
-  mask_mext (gsub arr (SZ.v i) (SZ.v j)) (fun k -> mask (k + SZ.v i));
-  rewrite each gsub arr (SZ.v i) (SZ.v j) as sub_impl arr (SZ.v i) (SZ.v j);
-  sub_impl arr (SZ.v i) (SZ.v j)
+  gsub_intro arr #f #(mask_isect mask pred) (SZ.v i) j;
+  mask_mext (gsub arr (SZ.v i) j) (fun k -> mask (k + SZ.v i));
+  rewrite each gsub arr (SZ.v i) j as sub_impl arr (SZ.v i) j;
+  sub_impl arr (SZ.v i) j
 }
 
 [@@allow_ambiguous]
