pulse/test/ExtractionTest.fst
@@ -128,7 +128,7 @@ fn sub_array (x: array U32.t)
   ensures pts_to x seq![0ul; 42ul]
 {
   to_mask x;
-  mask_write (Pulse.Lib.Array.sub x 1sz 2sz) 0sz 42ul;
+  mask_write (Pulse.Lib.Array.sub x 1sz 2) 0sz 42ul;
   return_sub x;
   mask_vext x seq![0ul; 42ul];
   from_mask x;
